Please split F before we hit line 2000

Clap/Lang/F/F.lean
@@ -9,7 +9,1068 @@ variable {p : ℕ}
 
 abbrev F := ExprRef
 abbrev FB := F
-abbrev FArray (k) := Vector FB k
+abbrev FArray (k) := Vector FB k -- TODO FB_Vector?
+abbrev FList := List FB
+
+section Converts
+
+namespace F
+
+abbrev toExprs (x : F) : List ExprRef := [x]
+abbrev serializeVal (x : ZMod p) : List (ZMod p) := [x]
+
+def Converts
+  (state : ClapMState p)
+  (expr : F)
+  (val : ZMod p)
+:=
+  Clap.Converts serializeVal state (toExprs expr) val
+
+def ConvertsM
+  (action : ClapM p F)
+:=
+  Clap.ConvertsM serializeVal (toExprs <$> action)
+
+end F
+
+
+namespace FB
+
+abbrev toExprs (x : FB) : List ExprRef := [x]
+abbrev serializeVal (x : Bool) : List (ZMod p) := [if x then 1 else 0]
+
+def Converts
+  (state : ClapMState p)
+  (expr : FB)
+  (val : Bool)
+:=
+  Clap.Converts serializeVal state (toExprs expr) val
+
+def ConvertsM
+  (action : ClapM p FB)
+:=
+  Clap.ConvertsM serializeVal (toExprs <$> action)
+
+end FB
+
+
+namespace FUnit
+
+abbrev toExprs (_ : Unit) : List ExprRef := []
+abbrev serializeVal (_ : Unit) : List (ZMod p) := []
+
+def Converts
+  (state : ClapMState p)
+  (expr : Unit)
+  (val : Unit)
+:=
+  Clap.Converts serializeVal state (toExprs expr) val
+
+def ConvertsM
+  (action : ClapM p Unit)
+:=
+  Clap.ConvertsM serializeVal (toExprs <$> action)
+
+end FUnit
+
+
+namespace FArray
+
+abbrev toExprs {k} (x : FArray k) : List ExprRef := x.toList
+abbrev serializeVal {k} (x : Vector Bool k) : List (ZMod p) := (x.map fun x ↦ if x then 1 else 0).toList
+
+def Converts
+  {k}
+  (state : ClapMState p)
+  (exprs : FArray k)
+  (vals : Vector Bool k)
+:=
+  Clap.Converts serializeVal state (toExprs exprs) vals
+
+def ConvertsM {k}
+  (action : ClapM p (FArray k))
+  (state : ClapMState p)
+  (vals : Vector Bool k)
+:=
+  Clap.ConvertsM serializeVal (toExprs <$> action) state vals
+
+end FArray
+
+
+namespace FList
+
+abbrev toExprs (x : FList) : List ExprRef := x
+abbrev serializeVal (x : List Bool) : List (ZMod p) := x.map fun x ↦ if x then 1 else 0
+
+def Converts
+  (state : ClapMState p)
+  (exprs : List FB)
+  (val : List Bool)
+:= Clap.Converts
+  (fun l : List Bool ↦ l.map fun x ↦ if x then 1 else 0)
+  state
+  exprs
+  val
+
+def ConvertsM
+  (action : ClapM p FList)
+  (state : ClapMState p)
+  (val : List Bool)
+:= Clap.ConvertsM
+  (fun l : List Bool ↦ l.map fun x ↦ if x then 1 else 0)
+  action
+  state
+  val
+
+end FList
+
+end Converts
+
+
+section ConvertsLemmas
+
+namespace F
+
+lemma converts_of_convertsM
+  {action : ClapM p F}
+  {state} {val}
+  (h : (ConvertsM action state val))
+:
+  Converts (action.getState state) (action.getResult state.numAlloc state.σ) val
+:= by
+  convert h.result
+  simp [Converts]
+
+structure Spec (state) where
+  action : ClapM p F
+  spec : ZMod p
+  converts : ConvertsM action state spec
+
+@[aesop unsafe apply]
+lemma converts_skip
+  {α} {conversion}
+  {skip : ClapM p (List ExprRef)} {state}
+  {val' : α} {expr : F} {val : ZMod p}
+  (h_skip : Clap.ConvertsM conversion skip state val')
+  (h : Converts state expr val)
+:
+  Converts (skip.getState state)
+           expr
+           val
+:=
+  Clap.converts_skip h_skip h
+
+@[aesop safe]
+lemma convertsM_pure
+        {state : ClapMState p}
+        {x : F}
+        {val : ZMod p}
+        (h : F.Converts state x val)
+  : ConvertsM (pure x) state val := by
+  constructor
+  · simpa
+  · grind
+  . simp [ClapM.runAndEval]
+
+lemma converts_of_FB_converts
+  {state : ClapMState p}
+  {expr : FB}
+  {b}
+  (h : FB.Converts state expr b)
+:
+  Converts state expr (if b then 1 else 0)
+:= by
+  obtain ⟨_, _, _, _⟩ := h
+  constructor <;> simp_all
+
+end F
+
+
+namespace FB
+
+lemma converts_of_convertsM
+  {action : ClapM p F}
+  {state} {val}
+  (h : (ConvertsM action state val))
+:
+  Converts (action.getState state) (action.getResult state.numAlloc state.σ) val
+:= by
+  convert h.result
+  simp [Converts]
+
+/-
+Best not to use because unification struggles to pick out function_val
+Instead, build forwards, applying action and function to the state in order
+-/
+lemma convertsM_bind_F
+  (action : ClapM p F)
+  (function : F → ClapM p FB)
+  (state)
+  {action_val : ZMod p}
+  (function_val : ZMod p → Bool)
+  (h_action : F.ConvertsM action state action_val)
+  (h_function : FB.ConvertsM
+    (function (action.getResult state.numAlloc state.σ))
+    (action.getState state)
+    (function_val action_val)
+  )
+:
+  ConvertsM (action >>= function) state (function_val action_val)
+:= by
+  constructor
+  . simp [ClapM.getState]
+    rewrite [ClapM.getVarStore_bind_of_wellFormed]
+    . apply h_function.result
+    . apply h_action.wellFormed
+    . apply h_function.wellFormed
+  . apply ClapM.bind_wellFormed
+    . apply h_action.wellFormed
+    . apply h_function.wellFormed
+  . obtain ⟨_,_,a_constraints⟩ := h_action
+    obtain ⟨_,_,f_constraints⟩ := h_function
+    grind [ClapM.getState]
+
+
+structure Spec (state) where
+  action : ClapM p FB
+  spec : Bool
+  converts : ConvertsM action state spec
+
+end FB
+
+
+namespace FArray
+
+lemma converts_of_convertsM
+  {k}
+  {action : ClapM p (FArray k)}
+  {state} {val}
+  (h : (ConvertsM action state val))
+:
+  Converts (action.getState state) (action.getResult state.numAlloc state.σ) val
+:= by
+  convert h.result
+  simp [Converts]
+
+lemma converts_skip
+  {k1} {α} {conversion}
+  {skip : ClapM p (List ExprRef)} {state}
+  {val : Vector Bool k1} {val' : α} {exprs : Vector ExprRef k1}
+  (h_skip : Clap.ConvertsM conversion skip state val')
+  (h : FArray.Converts state exprs val) :
+  FArray.Converts (skip.getState state)
+                   exprs
+                   val := by
+  rcases eq! : h
+  rcases h_skip
+  constructor
+  · grind [=Expr.varSet_wellFormed, ClapM.getState]
+  · grind [ClapM.getState]
+  next _ _ _ _ _ H _ =>
+    intro i
+    unfold ClapM.getState ClapM.getVarStore
+    rw [eval_varStore_eval_eq_some h]
+    exact H.2.2
+  · exact h.1
+
+lemma convertsM_bind_F
+  {k}
+  (action : ClapM p F)
+  (function : F → ClapM p (Vector ExprRef k))
+  (state)
+  {action_val : ZMod p}
+  (function_val : ZMod p → Vector Bool k)
+  (h_action : F.ConvertsM action state action_val)
+  (h_function : FArray.ConvertsM
+    (function (action.getResult state.numAlloc state.σ))
+    (action.getState state)
+    (function_val action_val)
+  )
+:
+  ConvertsM (action >>= function) state (function_val action_val)
+:= by
+  constructor
+  . simp [ClapM.getState]
+    rewrite [ClapM.getVarStore_bind_of_wellFormed]
+    . apply h_function.result
+    . apply h_action.wellFormed
+    . apply h_function.wellFormed
+  . apply ClapM.bind_wellFormed
+    . apply h_action.wellFormed
+    . apply h_function.wellFormed
+  . rewrite [Circuit.runAndEval_map_constraints, Circuit.runAndEval_bind_constraints]
+    . exact ⟨h_action.constraints, h_function.constraints⟩
+    . exact h_action.wellFormed
+    . grind [ClapM.getState, FArray.ConvertsM, cases Clap.ConvertsM]
+
+lemma convertsM_bind_FB
+  {k}
+  (action : ClapM p FB)
+  (function : FB → ClapM p (Vector ExprRef k))
+  (state)
+  {action_val : Bool}
+  (function_val : Bool → Vector Bool k)
+  (h_action : FB.ConvertsM action state action_val)
+  (h_function : FArray.ConvertsM
+    (function (action.getResult state.numAlloc state.σ))
+    (action.getState state)
+    (function_val action_val)
+  )
+:
+  ConvertsM (action >>= function) state (function_val action_val)
+:= by
+  constructor
+  . simp [ClapM.getState]
+    rewrite [ClapM.getVarStore_bind_of_wellFormed]
+    . apply h_function.result
+    . apply h_action.wellFormed
+    . apply h_function.wellFormed
+  . apply ClapM.bind_wellFormed
+    . apply h_action.wellFormed
+    . apply h_function.wellFormed
+  . rewrite [Circuit.runAndEval_map_constraints, Circuit.runAndEval_bind_constraints]
+    . exact ⟨h_action.constraints, h_function.constraints⟩
+    . exact h_action.wellFormed
+    . grind [ClapM.getState, FArray.ConvertsM, cases Clap.ConvertsM]
+
+lemma convertsM_bind_FArray
+  {k1 k2}
+  (action : ClapM p (Vector FB k1))
+  (function : Vector FB k1 → ClapM p (Vector FB k2))
+  (state)
+  {action_val : Vector Bool k1}
+  (function_val : Vector Bool k1 → Vector Bool k2)
+  (h_action : FArray.ConvertsM action state action_val)
+  (h_function : FArray.ConvertsM
+    (function (action.getResult state.numAlloc state.σ))
+    (action.getState state)
+    (function_val action_val)
+  )
+:
+  ConvertsM (action >>= function) state (function_val action_val)
+:= by
+  constructor
+  . simp [ClapM.getState]
+    rewrite [ClapM.getVarStore_bind_of_wellFormed]
+    . apply h_function.result
+    . apply h_action.wellFormed
+    . apply h_function.wellFormed
+  . apply ClapM.bind_wellFormed
+    . apply h_action.wellFormed
+    . apply h_function.wellFormed
+  . rewrite [Circuit.runAndEval_map_constraints, Circuit.runAndEval_bind_constraints]
+    . exact ⟨h_action.constraints, h_function.constraints⟩
+    . exact h_action.wellFormed
+    . grind [ClapM.getState, FArray.ConvertsM, cases Clap.ConvertsM]
+
+lemma convertsM_map_FB_FArray
+  {k}
+  (action : ClapM p FB)
+  (f : FB → Vector FB k)
+  (state)
+  {action_val : Bool}
+  (f_val : Bool → Vector Bool k)
+  (h_action : FB.ConvertsM action state action_val)
+  (h_f_val : FArray.Converts
+    (action.getState state)
+    (f (action.getResult state.numAlloc state.σ))
+    (f_val action_val)
+  )
+:
+  ConvertsM (f <$> action) state (f_val action_val)
+:= by
+  constructor
+  . simp
+    apply h_f_val
+  . rewrite [ClapM.map_wellFormed]
+    apply h_action.wellFormed
+  . simp [ClapM.runAndEval]
+    exact h_action.constraints
+
+@[aesop safe]
+lemma convertsM_pure
+        {k}
+        {state : ClapMState p}
+        {x : Vector ExprRef k}
+        {val : Vector Bool k}
+        (h : FArray.Converts state x val)
+  : ConvertsM (pure x) state val := by
+  constructor
+  · simpa
+  · grind
+  . simp [ClapM.runAndEval]
+
+@[simp]
+lemma converts_empty
+        {state : ClapMState p}
+  : Converts state #v[] #v[] := by
+  constructor
+  . simp
+  · simp
+  · grind
+  · grind
+
+lemma converts_push
+  {k}
+  {state : ClapMState p}
+  {exprs : Vector FB k}
+  {expr : FB}
+  {vals : Vector Bool k}
+  {val : Bool}
+  (h_exprs : FArray.Converts state exprs vals)
+  (h_expr : FB.Converts state expr val)
+:
+  FArray.Converts state (exprs.push expr) (vals.push val)
+:= by
+  obtain ⟨exprs_length, exprs_varSet, exprs_wellFormed, exprs_result⟩ := h_exprs
+  obtain ⟨expr_lengh, expr_varSet, expr_wellFormed, expr_result⟩ := h_expr
+  simp at *
+  constructor
+  . intro i
+    simp [Vector.getElem_push]
+    split
+    . exact exprs_varSet ⟨i.val, by grind⟩
+    . assumption
+  . intro i
+    simp [Vector.getElem_push]
+    split
+    . exact exprs_wellFormed ⟨i.val, by grind⟩
+    . assumption
+  . intro i
+    simp [Vector.getElem_push]
+    split
+    . exact exprs_result ⟨i.val, by grind⟩
+    . assumption
+  . grind
+
+lemma convertsM_of_convertsM_toList
+  {k}
+  {action : ClapM p (Vector FB k)}
+  {state}
+  {val : Vector Bool k}
+  (h : FList.ConvertsM (Vector.toList <$> action) state val.toList)
+:
+  FArray.ConvertsM action state val
+:= by
+  constructor
+  . obtain ⟨⟨_, _, _, _⟩, _, _⟩ := h
+    constructor <;> simp at *
+    . assumption
+    . assumption
+    . assumption
+  . grind [h.wellFormed]
+  . grind [h.constraints, ClapM.runAndEval]
+
+lemma converts_cast
+  {k1 k2}
+  {state : ClapMState p}
+  {exprs : FArray k1}
+  {val : Vector Bool k1}
+  (h : FArray.Converts state exprs val)
+  (h_k : k1 = k2)
+:
+  FArray.Converts state (exprs.cast h_k) (val.cast h_k)
+:= by
+  obtain ⟨h_len, h_varSet, h_wf, h_value⟩ := h
+  constructor
+  . intro i
+    specialize h_varSet ⟨i.val, by grind⟩
+    simp at ⊢ h_varSet
+    convert h_varSet
+    grind
+  . intro i
+    specialize h_wf ⟨i.val, by grind⟩
+    simp at ⊢ h_wf
+    convert h_wf
+    grind
+  . intro i
+    specialize h_value ⟨i.val, by grind⟩
+    simp at ⊢ h_value
+    convert h_value
+    . grind
+    . grind
+  . grind
+
+lemma converts_pop
+  {k}
+  {state : ClapMState p}
+  {exprs : FArray k}
+  {val : Vector Bool k}
+  (h : FArray.Converts state exprs val)
+:
+  FArray.Converts state (exprs.pop) (val.pop)
+:= by
+  obtain ⟨h_len, h_varSet, h_wf, h_value⟩ := h
+  constructor
+  . intro i
+    specialize h_varSet ⟨i.val, by grind⟩
+    simp at ⊢ h_varSet
+    convert h_varSet
+  . intro i
+    specialize h_wf ⟨i.val, by grind⟩
+    simp at ⊢ h_wf
+    convert h_wf
+  . intro i
+    specialize h_value ⟨i.val, by grind⟩
+    simp at ⊢ h_value
+    convert h_value
+  . grind
+
+lemma converts_getElem
+  {k i}
+  {state : ClapMState p}
+  {exprs : FArray k}
+  {vals : Vector Bool k}
+  (h : FArray.Converts state exprs vals)
+  (h_i : i < k)
+:
+  FB.Converts state exprs[i] vals[i]
+:= by
+  obtain ⟨h_len, h_varSet, h_wf, h_value⟩ := h
+  constructor
+  . intro ib
+    specialize h_varSet ⟨i, by grind⟩
+    simp at ⊢ h_varSet
+    convert h_varSet
+  . intro ib
+    specialize h_wf ⟨i, by grind⟩
+    simp at ⊢ h_wf
+    convert h_wf
+  . intro ib
+    specialize h_value ⟨i, by grind⟩
+    simp at ⊢ h_value
+    convert h_value
+  . grind
+
+end FArray
+
+
+namespace FList
+
+lemma converts_of_convertsM
+  {action : ClapM p FList}
+  {state} {val}
+  (h : (ConvertsM action state val))
+:
+  Converts (action.getState state) (action.getResult state.numAlloc state.σ) val
+:= by
+  convert h.result
+  simp [Converts]
+
+@[aesop safe]
+lemma convertsM_pure
+        {state : ClapMState p}
+        {x : List FB}
+        {val : List Bool}
+        (h : FList.Converts state x val)
+  : ConvertsM (pure x) state val := by
+  constructor
+  · simpa
+  · grind
+  . grind [ClapM.runAndEval]
+
+@[simp]
+lemma converts_empty
+        {state : ClapMState p}
+  : Converts state [] [] := by
+  constructor
+  . simp
+  · simp
+  · grind
+  · grind
+
+lemma converts_skip
+  {α} {conversion}
+  {skip : ClapM p (List ExprRef)} {state}
+  {val' : α} {expr : List FB} {val : List Bool}
+  (h_skip : Clap.ConvertsM conversion skip state val')
+  (h : FList.Converts state expr val) :
+  FList.Converts (skip.getState state)
+             expr
+             val := toIdeal_run_of_toIdeal _ h_skip.wellFormed h
+
+lemma converts_append
+  {state : ClapMState p}
+  {exprs1 exprs2 : List FB}
+  {vals1 vals2 : List Bool}
+  (h_exprs1 : FList.Converts state exprs1 vals1)
+  (h_exprs2 : FList.Converts state exprs2 vals2)
+:
+  FList.Converts state (exprs1 ++ exprs2) (vals1 ++ vals2)
+:= by
+  obtain ⟨exprs1_length, exprs1_varSet, exprs1_wellFormed, exprs1_result⟩ := h_exprs1
+  obtain ⟨exprs2_lengh, exprs2_varSet, exprs2_wellFormed, exprs2_result⟩ := h_exprs2
+  simp at *
+  constructor
+  . intro i
+    simp [List.getElem_append]
+    split
+    . exact exprs1_varSet ⟨i.val, by grind⟩
+    . exact exprs2_varSet ⟨_, by grind⟩
+  . intro i
+    simp [List.getElem_append]
+    split
+    . exact exprs1_wellFormed ⟨i.val, by grind⟩
+    . exact exprs2_wellFormed ⟨_, by grind⟩
+  . intro i
+    simp [List.getElem_append, exprs1_length]
+    split
+    . exact exprs1_result ⟨i.val, by grind⟩
+    . exact exprs2_result ⟨_, by grind⟩
+  . grind
+
+lemma converts_of_converts_FB
+  {state : ClapMState p}
+  {exprs}
+  {vals}
+  (h_length : exprs.length = vals.length)
+  (h_converts : ∀ i : Fin exprs.length, FB.Converts state exprs[i] vals[i])
+:
+  FList.Converts state exprs vals
+:= by
+  constructor
+  . intro i
+    have := (h_converts i).varSet_wf
+    simp at this
+    assumption
+  . intro i
+    have := (h_converts i).expr_wf
+    simp at this
+    assumption
+  . intro i
+    have := (h_converts i).value_eq
+    simp at this
+    simp [this]
+  . grind
+
+lemma converts_singleton_of_converts_FB
+  {state : ClapMState p}
+  {expr}
+  {val}
+  (h_converts : FB.Converts state expr val)
+:
+  FList.Converts state [expr] [val]
+:= by
+  apply converts_of_converts_FB
+  . simpa
+  . simp
+
+end FList
+
+end ConvertsLemmas
+
+
+namespace eq0
+
+lemma wellFormed {e! : ExprRef} {state} {value : ZMod p}
+  (h : F.Converts state e! value)
+:
+  (eq0 e!).wellFormed state.numAlloc state.varStore state.σ
+:= by
+  obtain ⟨h_varSet, h_wellFormed, h_result⟩ := h
+  simp at *
+  apply wellFormed_eq0
+  . grind
+  . have : [state.varStore|⦃e!, state.σ⦄].isSome = true := by grind
+    grind
+  . grind
+
+lemma converts
+  [p.AtLeastTwo]
+  {state : ClapMState p}
+  {a : F}
+:
+  FUnit.Converts
+    ((eq0 a).getState state)
+    ((eq0 a).getResult state.numAlloc state.σ)
+    ()
+:= by
+  constructor <;> simp at *
+
+lemma constraints
+  {state : ClapMState p}
+  {a}
+  (h_a : F.Converts state a (0 : ZMod p))
+:
+  ((eq0 a).runAndEval state.numAlloc state.varStore state.σ).2.constraints
+:= by
+  simp
+  have := h_a.value_eq
+  simp at this
+  exact this
+
+lemma convertsM
+  [p.AtLeastTwo]
+  {state}
+  {a : F}
+  (h_a : F.Converts state a (0 : ZMod p))
+:
+  FUnit.ConvertsM (eq0 a)
+    state
+    ()
+where
+  result := converts
+  wellFormed := wellFormed h_a
+  constraints := constraints h_a
+
+end eq0
+
+
+namespace isZero
+
+@[simp, grind! .]
+lemma lt_getNumAlloc
+  {numAlloc : ℕ}
+  {σ : HashConsSt p}
+  {a : ExprRef}
+:
+  numAlloc < (isZero a).getNumAlloc numAlloc σ
+:= by
+  simp [isZero]
+
+lemma wellFormed {e! : ExprRef} {state} {value : ZMod p}
+  (h : F.Converts state e! value)
+:
+  (isZero e!).wellFormed state.numAlloc state.varStore state.σ
+:= by
+  obtain ⟨h_varSet, h_wellFormed, h_result⟩ := h
+  simp at *
+  apply wellFormed_isZero
+  . grind
+  . have : [state.varStore|⦃e!, state.σ⦄].isSome = true := by grind
+    grind
+  . grind
+
+lemma converts
+  [p.AtLeastTwo]
+  {state}
+  {a : F}
+  {a_val : ZMod p}
+  (h_a : F.Converts state a a_val)
+:
+  FB.Converts
+    ((isZero a).getState state)
+    ((isZero a).getResult state.numAlloc state.σ)
+    (a_val == 0)
+:= by
+  obtain ⟨a_length, a_varSet, a_wellFormed, a_result⟩ := h_a
+  obtain ⟨varStore, σ, numAlloc⟩ := state
+  simp [ClapM.getState]
+  constructor <;> simp at *
+  . intro i h_i
+    grind [=isZero, ClapM.getState]
+  . simp [isZero]
+    rw [Expr.wellFormed_iff_isSome, Expr.deref_mkVar_eq_some]
+    rfl
+  . simp [isZero, HashConsM.mkVar]
+    simp [HashConsM.getHashConsState_saveExpr_of_wellFormed,
+          HashConsM.getResult_saveExpr_of_wellFormed]
+    split
+    · rw [eval_eq_evalRec (by grind)]
+      unfold Expr.evalRec
+      grind
+    · rw [eval_eq_evalRec (by grind)]
+      rw [evalRec_eq_of_deref_eq_some_v (idx := numAlloc)]
+      · simp
+        rw [eval_eq_evalRec (by grind)] at a_result ⊢
+        rw [←evalRec_of_wellFormed_of_prefix] at ⊢
+        · rw [a_result]
+          grind
+        · grind
+        · grind
+      · grind
+
+lemma constraints
+  {state : ClapMState p}
+  {a}
+  {a_val}
+  (h_a : F.Converts state a a_val)
+:
+  ((isZero a).runAndEval state.numAlloc state.varStore state.σ).2.constraints
+:= by
+  simp
+  have : [state.varStore|⦃a, state.σ⦄].isSome := by grind [F.Converts]
+  exact isSome_eval_of_prefix (by {
+    grind [F.Converts, cases Converts]
+  }) this (by rfl) (by grind)
+
+lemma convertsM
+  [p.AtLeastTwo]
+  {state}
+  {a : F}
+  {a_val : ZMod p}
+  (h_a : F.Converts state a a_val)
+:
+  FB.ConvertsM (isZero a)
+    state
+    (a_val == 0)
+where
+  result := converts h_a
+  wellFormed := wellFormed h_a
+  constraints := constraints h_a
+
+def spec [p.AtLeastTwo]
+  {a : F} {state : ClapMState p} {a_val}
+  (h: (F.Converts state a a_val))
+:
+  FB.Spec state
+where
+  action := isZero a
+  spec := a_val == 0
+  converts := convertsM h
+
+end isZero
+
+
+namespace mkAdd
+
+lemma converts
+   {state}
+   {a b : ExprRef}
+   {a_val b_val : ZMod p}
+   (h_a : F.Converts state a a_val)
+   (h_b : F.Converts state b b_val)
+:
+  F.Converts
+    (ClapM.getState (liftM (HashConsM.mkAdd (p := p) a b)) state)
+    (ClapM.getResult (liftM (HashConsM.mkAdd (p := p) a b)) state.numAlloc state.σ)
+    (a_val + b_val)
+:= by
+  simp [ClapM.getState]
+  obtain ⟨a_length, a_varSet, a_wellFormed, a_result⟩ := h_a
+  obtain ⟨b_length, b_varSet, b_wellFormed, b_result⟩ := h_b
+  constructor <;>
+  simp at *
+  . grind [=Expr.varSet_wellFormed]
+  . grind
+  . grind
+
+lemma constraints
+  {state : ClapMState p}
+  {a b}
+:
+  ((liftM (n := ClapM p) (HashConsM.mkAdd (p := p) a b)).runAndEval state.numAlloc state.varStore state.σ).2.constraints
+:= by
+  grind [ClapM.runAndEval]
+
+lemma convertsM
+  {state}
+  {a b : ExprRef}
+  {a_val b_val : ZMod p}
+  (h_a : F.Converts state a a_val)
+  (h_b : F.Converts state b b_val)
+:
+  F.ConvertsM (liftM (HashConsM.mkAdd (p := p) a b)) state (a_val + b_val)
+where
+  result := converts h_a h_b
+  wellFormed := ClapM.wellFormed_liftM_of_hashConsM_wellFormed HashConsM.wellFormed_mkAdd
+  constraints := constraints
+
+def spec
+  {a b : F} {state : ClapMState p} {a_val b_val}
+  (h_a: (F.Converts state a a_val))
+  (h_b: (F.Converts state b b_val))
+:
+  F.Spec state
+where
+  action := (liftM (HashConsM.mkAdd (p := p) a b))
+  spec := a_val + b_val
+  converts := convertsM h_a h_b
+
+end mkAdd
+
+
+namespace mkSub
+
+lemma converts
+   {state}
+   {a b : ExprRef}
+   {a_val b_val : ZMod p}
+   (h_a : F.Converts state a a_val)
+   (h_b : F.Converts state b b_val)
+:
+  F.Converts
+    (ClapM.getState (liftM (HashConsM.mkSub (p := p) a b)) state)
+    (ClapM.getResult (liftM (HashConsM.mkSub (p := p) a b)) state.numAlloc state.σ)
+    (a_val - b_val)
+:= by
+  simp [ClapM.getState]
+  obtain ⟨a_length, a_varSet, a_wellFormed, a_result⟩ := h_a
+  obtain ⟨b_length, b_varSet, b_wellFormed, b_result⟩ := h_b
+  constructor <;>
+  simp at *
+  . grind [=Expr.varSet_wellFormed]
+  . grind
+  . grind
+
+lemma constraints
+  {state : ClapMState p}
+  {a b}
+:
+  ((liftM (n := ClapM p) (HashConsM.mkSub (p := p) a b)).runAndEval state.numAlloc state.varStore state.σ).2.constraints
+:= by
+  grind [ClapM.runAndEval]
+
+lemma convertsM
+  {state}
+  {a b : ExprRef}
+  {a_val b_val : ZMod p}
+  (h_a : F.Converts state a a_val)
+  (h_b : F.Converts state b b_val)
+:
+  F.ConvertsM (liftM (HashConsM.mkSub (p := p) a b)) state (a_val - b_val)
+where
+  result := converts h_a h_b
+  wellFormed := ClapM.wellFormed_liftM_of_hashConsM_wellFormed HashConsM.wellFormed_mkSub
+  constraints := constraints
+
+def spec
+  {a b : F} {state : ClapMState p} {a_val b_val}
+  (h_a: (F.Converts state a a_val))
+  (h_b: (F.Converts state b b_val))
+:
+  F.Spec state
+where
+  action := (liftM (HashConsM.mkSub (p := p) a b))
+  spec := a_val - b_val
+  converts := convertsM h_a h_b
+
+end mkSub
+
+
+namespace mkMul
+
+lemma converts
+   {state}
+   {a b : ExprRef}
+   {a_val b_val : ZMod p}
+   (h_a : F.Converts state a a_val)
+   (h_b : F.Converts state b b_val)
+:
+  F.Converts
+    (ClapM.getState (liftM (HashConsM.mkMul (p := p) a b)) state)
+    (ClapM.getResult (liftM (HashConsM.mkMul (p := p) a b)) state.numAlloc state.σ)
+    (a_val * b_val)
+:= by
+  simp [ClapM.getState]
+  obtain ⟨a_length, a_varSet, a_wellFormed, a_result⟩ := h_a
+  obtain ⟨b_length, b_varSet, b_wellFormed, b_result⟩ := h_b
+  constructor <;>
+  simp at *
+  . grind [=Expr.varSet_wellFormed]
+  . grind
+  . grind
+
+lemma constraints
+  {state : ClapMState p}
+  {a b}
+:
+  ((liftM (n := ClapM p) (HashConsM.mkMul (p := p) a b)).runAndEval state.numAlloc state.varStore state.σ).2.constraints
+:= by
+  grind [ClapM.runAndEval]
+
+lemma convertsM
+  {state}
+  {a b : ExprRef}
+  {a_val b_val : ZMod p}
+  (h_a : F.Converts state a a_val)
+  (h_b : F.Converts state b b_val)
+:
+  F.ConvertsM (liftM (HashConsM.mkMul (p := p) a b)) state (a_val * b_val)
+where
+  result := converts h_a h_b
+  wellFormed := ClapM.wellFormed_liftM_of_hashConsM_wellFormed HashConsM.wellFormed_mkMul
+  constraints := constraints
+
+def spec
+  {a b : F} {state : ClapMState p} {a_val b_val}
+  (h_a: (F.Converts state a a_val))
+  (h_b: (F.Converts state b b_val))
+:
+  F.Spec state
+where
+  action := (liftM (HashConsM.mkMul (p := p) a b))
+  spec := a_val * b_val
+  converts := convertsM h_a h_b
+
+end mkMul
+
+
+section eq
+
+def eq {p : ℕ} [p.AtLeastTwo] (a b : F) : ClapM p FB := do
+  isZero (←HashConsM.mkSub (p := p) a b)
+
+namespace eq
+
+lemma convertsM
+  [p.AtLeastTwo]
+  {state}
+  {a b : F}
+  {a_val b_val : ZMod p}
+  (h_a : F.Converts state a a_val)
+  (h_b : F.Converts state b b_val)
+:
+  FB.ConvertsM (eq a b) state (a_val == b_val)
+:= by
+  unfold eq
+
+  have this := mkSub.convertsM h_a h_b
+  have h_wf := this.wellFormed
+  have h_constraints := this.constraints
+  have := isZero.convertsM (F.converts_of_convertsM this)
+  have h_wf := this.wellFormed
+  have h_constraints := this.constraints
+  constructor
+  . convert this.result using 1
+    . grind
+    . grind [ClapM.getState]
+    . grind
+  . grind [ClapM.getState]
+  . grind [ClapM.getState]
+
+end eq
+end eq
+
+
+namespace MkConstant
+
+@[simp]
+lemma convertsM
+  {state}
+  {x : ZMod p}
+:
+  F.ConvertsM (liftM (HashConsM.mkConstant (p := p) x)) state x
+:= by
+  constructor
+  · simp [ClapM.getState]
+    simp_rw [HashConsM.getResult_mkConstant, HashConsM.getHashConsState_mkConstant]
+    constructor <;> simp
+    · grind [=Expr.varSet, =Expr.varSet_wellFormed]
+    · grind
+    · rw [eval_eq_evalRec (by grind)]
+      grind
+  · grind
+  . grind [ClapM.runAndEval]
+
+def spec
+  (x : ZMod p)
+  (state : ClapMState p)
+:
+  F.Spec state
+where
+  action := (liftM (HashConsM.mkConstant (p := p) x))
+  spec := x
+  converts := convertsM
+
+-- TODO, see if this can be done generally?
+lemma fold_spec {x : ZMod p} (state : ClapMState p):
+  (liftM (HashConsM.mkConstant (p := p) x)) =
+  (spec x state).action
+:= rfl
+
+end MkConstant
+
 
 section OneHotRaw
 
@@ -17,27 +1078,11 @@ open HashConsM
 
 variable {p : ℕ} [p.AtLeastTwo] {start len : ℕ} {idx : F} {numAlloc : ℕ} {σ : HashConsSt p}
 
-def eq {p : ℕ} [p.AtLeastTwo] (a b : F) : ClapM p FB := do
-  isZero (←mkSub (p := p) a b)
-
 def oneHotRaw_aux (start len : ℕ) (idx : F) : ClapM p (Vector FB len) :=
   (Vector.range' start len).mapM (fun (i:ℕ) ↦ do
     let idx_val ← mkConstant (p := p) i
     eq idx idx_val
   )
-
--- /--
--- Yeah ok...
-
--- TODO: Remove (here to save build time)
--- -/
--- @[simp, grind =]
---lemma _root_.Vector.mapM_singleton {m : Type → Type} [Monad m] [LawfulMonad m]
---   {α β : Type}
---   {f : α → m β} {x} :
---   #v[x].mapM f = f x >>= (pure #v[·]) := by
---   rw [←map_inj_right (f := Vector.toArray) (by aesop)]
---   simp
 
 @[simp, grind =]
 lemma oneHotRaw_aux_zero :
@@ -62,7 +1107,7 @@ lemma oneHotRaw_aux_succ :
   rw [←oneHotRaw_aux.eq_def]
   simp
 
-def oneHotRaw (len : ℕ) (idx : F) : ClapM p (Vector FB len) :=
+def oneHotRaw (len : ℕ) (idx : F) : ClapM p (FArray len) :=
   oneHotRaw_aux 0 len idx
 
 def oneHotRaw'_aux (start len : ℕ) (idx : F) : ClapM p (List FB) :=
@@ -154,1111 +1199,33 @@ lemma toList_map_oneHotRaw_eq_oneHotRaw' :
   Vector.toList <$> (oneHotRaw (p := p) len idx) =
   oneHotRaw' len idx := toList_map_oneHotRaw_aux_eq_oneHotRaw'_aux
 
-end OneHotRaw
-
-namespace F
-
-def Converts
-  (state : ClapMState p)
-  (expr : F)
-  (val : ZMod p)
-:=
-  Clap.Converts' (fun x : ZMod p ↦ [x]) state [expr] val
-
-structure ConvertsM
-  (action : ClapM p F)
-  (state : ClapMState p)
-  (val : ZMod p)
-: Prop where
-  result : Converts
-    (action.getState state)
-    (action.getResult state.numAlloc state.σ)
-    val
-  wellFormed : action.wellFormed state.numAlloc state.varStore state.σ
-  -- constraints : [state.varStore, (action.getState state).σ, state.numAlloc|action.getCircuit state.numAlloc state.σ]ₑ.constraints
-
-structure Spec (state) where
-  action : ClapM p F
-  spec : ZMod p
-  converts : ConvertsM action state spec
-
-end F
-
-namespace FB
-
-def Converts
-  (state : ClapMState p)
-  (expr : FB)
-  (val : Bool)
-:=
-  Clap.Converts' (fun x : Bool ↦ [if x then (1 : ZMod p) else 0]) state [expr] val
-
-structure ConvertsM
-  (action : ClapM p FB)
-  (state : ClapMState p)
-  (val : Bool)
-: Prop where
-  result : Converts
-    (action.getState state)
-    (action.getResult state.numAlloc state.σ)
-    val
-  wellFormed : action.wellFormed state.numAlloc state.varStore state.σ
-  -- constraints : [state.varStore, (action.getState state).σ, state.numAlloc|action.getCircuit state.numAlloc state.σ]ₑ.constraints
-
-lemma convertsM_of_convertsM_eq
-  {action : ClapM p FB}
-  {state val₁}
-  (val₂ : Bool)
-  (h : ConvertsM action state val₂)
-  (h_eq : val₁ = val₂)
-:
-  ConvertsM action state val₁
-where
-  result := by rewrite [h_eq]; exact h.result
-  wellFormed := h.wellFormed
-
-class ToIdeal (α : Type) where
-  toIdeal : Type
-
-instance : ToIdeal FB where
-  toIdeal := Bool
-
--- TODO generalise
-lemma convertsM_bind
-  (action : ClapM p F)
-  (function : F → ClapM p FB)
-  (state)
-  {action_val : ZMod p}
-  (function_val : ZMod p → Bool)
-  (h_action : F.ConvertsM action state action_val)
-  (h_function : FB.ConvertsM
-    (function (action.getResult state.numAlloc state.σ))
-    (action.getState state)
-    (function_val action_val)
-  )
-:
-  ConvertsM (action >>= function) state (function_val action_val)
-:= by
-  constructor
-  . simp [ClapM.getState]
-    rewrite [ClapM.getVarStore_bind_of_wellFormed]
-    . apply h_function.result
-    . apply h_action.wellFormed
-    . apply h_function.wellFormed
-  . apply ClapM.bind_wellFormed
-    . apply h_action.wellFormed
-    . apply h_function.wellFormed
-
-structure Spec (action : ClapM p FB) (state) where
-  spec : Bool
-  converts : ConvertsM action state spec
-
-end FB
-
-
-namespace FArray
-
-def Converts (k : ℕ) := Clap.Converts k
-  fun vec : Vector Bool k ↦ vec.map fun x ↦ if x then (1 : ZMod p) else 0
-
-def Converts'
-  {k}
-  (state : ClapMState p)
-  (exprs : Vector FB k)
-  (val : Vector Bool k)
-:= Clap.Converts'
-  (fun l : List Bool ↦ l.map fun x ↦ if x then 1 else 0)
-  state
-  exprs.toList
-  val.toList
-
-
-@[aesop unsafe apply, grind .]
-lemma converts_of_converts' {k} {state : ClapMState p}
-  {exprs : Vector ExprRef k} {val : Vector Bool k}
-  (h : Converts' state exprs val) :
-  Converts k state exprs val := by
-  unfold Converts
-  unfold Converts' at h
-  rcases h with ⟨h₁, h₂, h₃, h₄⟩
-  have : exprs.toList.length = k := by aesop
-  rw! (castMode := .all) [this] at h₁ h₂ h₃ h₄
-  constructor <;> intros i <;>
-  · specialize_all i
-    grind
-
-structure ConvertsM {k}
-  (action : ClapM p (Vector FB k))
-  (state)
-  (val : Vector Bool k)
-: Prop where
-  result : Converts k
-    (action.getState state)
-    (action.getResult state.numAlloc state.σ)
-    val
-  wellFormed : action.wellFormed state.numAlloc state.varStore state.σ
-  -- constraints : [state.varStore, (action.getState state).σ, state.numAlloc|action.getCircuit state.numAlloc state.σ]ₑ.constraints
-
-lemma ConvertsM.def {k state} {action : ClapM p (Vector FB k)}
-                    {val : Vector Bool k}:
-  ConvertsM action state val ↔
-  Converts k
-    (action.getState state)
-    (action.getResult state.numAlloc state.σ)
-    val ∧
-  action.wellFormed state.numAlloc state.varStore state.σ := by
-  apply Iff.intro <;> intros h
-  rcases h
-  grind
-  constructor
-  grind
-  grind
-
-structure ConvertsM'
-  {k}
-  (action : ClapM p (Vector FB k))
-  (state)
-  (val : Vector Bool k)
-: Prop where
-  result : Converts'
-    (action.getState state)
-    (action.getResult state.numAlloc state.σ)
-    val
-  wellFormed : action.wellFormed state.numAlloc state.varStore state.σ
-  -- constraints : [state.varStore, (action.getState state).σ, state.numAlloc|action.getCircuit state.numAlloc state.σ]ₑ.constraints
-
-lemma ConvertsM'.def {k} {state} {action : ClapM p (Vector FB k)}
-                     {val : Vector Bool k}
-:
-  ConvertsM' action state val ↔
-  Converts'
-    (action.getState state)
-    (action.getResult state.numAlloc state.σ)
-    val ∧
-  action.wellFormed state.numAlloc state.varStore state.σ := by
-  apply Iff.intro <;> intros h
-  rcases h
-  grind
-  constructor
-  grind
-  grind
-
-@[aesop unsafe apply, grind =>]
-lemma converts'_skip
-  {k1 k2}
-  {skip : ClapM p (Vector FB k2)} {state}
-  {val : Vector Bool k1} {val' : Vector Bool k2} {exprs : Vector ExprRef k1}
-  (h_skip : FArray.ConvertsM' skip state val')
-  (h : FArray.Converts' state exprs val) :
-  FArray.Converts' (skip.getState state)
-                   exprs
-                   val := by
-  rcases eq! : h
-  rcases h_skip
-  constructor
-  · grind [=Expr.varSet_wellFormed, ClapM.getState]
-  · grind [ClapM.getState]
-  next _ _ _ _ _ H =>
-    intro i
-    unfold ClapM.getState ClapM.getVarStore
-    rw [eval_varStore_eval_eq_some' h]
-    exact H.2.2
-  · exact h.1
-
-@[aesop unsafe apply, grind =>]
-lemma converts'_skip_FB
-  {k}
-  {skip : ClapM p FB} {state} {val : Vector Bool k} {val' : Bool} {exprs : Vector ExprRef k}
-  (h_skip : FB.ConvertsM skip state val')
-  (h : FArray.Converts' state exprs val) :
-  FArray.Converts' (skip.getState state)
-                   exprs
-                   val := by
-  rcases eq! : h
-  rcases h_skip
-  constructor
-  · grind [=Expr.varSet_wellFormed, ClapM.getState]
-  · grind [ClapM.getState]
-  next _ _ _ _ _ H =>
-    intro i
-    unfold ClapM.getState ClapM.getVarStore
-    rw [eval_varStore_eval_eq_some' h]
-    exact H.2.2
-  · exact h.1
-
-@[aesop unsafe apply, grind =>]
-lemma converts'_skip_F
-  {k}
-  {skip : ClapM p F} {state} {val : Vector Bool k} {val' : ZMod p} {exprs : Vector ExprRef k}
-  (h_skip : F.ConvertsM skip state val')
-  (h : FArray.Converts' state exprs val) :
-  FArray.Converts' (skip.getState state)
-                   exprs
-                   val := by
-  rcases eq! : h
-  rcases h_skip
-  constructor
-  · grind [=Expr.varSet_wellFormed, ClapM.getState]
-  · grind [ClapM.getState]
-  next _ _ _ _ _ H =>
-    intro i
-    unfold ClapM.getState ClapM.getVarStore
-    rw [eval_varStore_eval_eq_some' h]
-    exact H.2.2
-  · exact h.1
-
-@[aesop unsafe apply, grind .]
-lemma convertsM_of_ConvertsM' {k : ℕ} {state} {val : Vector Bool k}
-                              {action : ClapM p (Vector FB k)}
-                              (h : ConvertsM' action state val) :
-  ConvertsM action state val := by
-  rw [ConvertsM.def]; rw [ConvertsM'.def] at h
-  grind [ClapM.getState]
-
--- TODO generalise
-lemma convertsM_bind
-  {len1 len2}
-  (action : ClapM p (FArray len1))
-  (function : (FArray len1) → ClapM p (FArray len2))
-  (state)
-  {action_val : Vector Bool len1}
-  (function_val : Vector Bool len1 → Vector Bool len2)
-  (h_action : FArray.ConvertsM action state action_val)
-  (h_function : FArray.ConvertsM
-    (function (action.getResult state.numAlloc state.σ))
-    (action.getState state)
-    (function_val action_val)
-  )
-:
-  ConvertsM (action >>= function) state (function_val action_val)
-:= by
-  constructor
-  . simp [ClapM.getState]
-    rewrite [ClapM.getVarStore_bind_of_wellFormed]
-    . apply h_function.result
-    . apply h_action.wellFormed
-    . apply h_function.wellFormed
-  . apply ClapM.bind_wellFormed
-    . apply h_action.wellFormed
-    . apply h_function.wellFormed
-
-lemma convertsM'_bind_F
-  {k}
-  (action : ClapM p F)
-  (function : F → ClapM p (Vector ExprRef k))
-  (state)
-  {action_val : ZMod p}
-  (function_val : ZMod p → Vector Bool k)
-  (h_action : F.ConvertsM action state action_val)
-  (h_function : FArray.ConvertsM'
-    (function (action.getResult state.numAlloc state.σ))
-    (action.getState state)
-    (function_val action_val)
-  )
-:
-  ConvertsM' (action >>= function) state (function_val action_val)
-:= by
-  constructor
-  . simp [ClapM.getState]
-    rewrite [ClapM.getVarStore_bind_of_wellFormed]
-    . apply h_function.result
-    . apply h_action.wellFormed
-    . apply h_function.wellFormed
-  . apply ClapM.bind_wellFormed
-    . apply h_action.wellFormed
-    . apply h_function.wellFormed
-
-lemma convertsM'_bind_FB
-  {k}
-  (action : ClapM p FB)
-  (function : FB → ClapM p (Vector ExprRef k))
-  (state)
-  {action_val : Bool}
-  (function_val : Bool → Vector Bool k)
-  (h_action : FB.ConvertsM action state action_val)
-  (h_function : FArray.ConvertsM'
-    (function (action.getResult state.numAlloc state.σ))
-    (action.getState state)
-    (function_val action_val)
-  )
-:
-  ConvertsM' (action >>= function) state (function_val action_val)
-:= by
-  constructor
-  . simp [ClapM.getState]
-    rewrite [ClapM.getVarStore_bind_of_wellFormed]
-    . apply h_function.result
-    . apply h_action.wellFormed
-    . apply h_function.wellFormed
-  . apply ClapM.bind_wellFormed
-    . apply h_action.wellFormed
-    . apply h_function.wellFormed
-
-lemma convertsM'_bind_FArray
-  {k1 k2}
-  (action : ClapM p (Vector FB k1))
-  (function : Vector FB k1 → ClapM p (Vector FB k2))
-  (state)
-  {action_val : Vector Bool k1}
-  (function_val : Vector Bool k1 → Vector Bool k2)
-  (h_action : FArray.ConvertsM' action state action_val)
-  (h_function : FArray.ConvertsM'
-    (function (action.getResult state.numAlloc state.σ))
-    (action.getState state)
-    (function_val action_val)
-  )
-:
-  ConvertsM' (action >>= function) state (function_val action_val)
-:= by
-  constructor
-  . simp [ClapM.getState]
-    rewrite [ClapM.getVarStore_bind_of_wellFormed]
-    . apply h_function.result
-    . apply h_action.wellFormed
-    . apply h_function.wellFormed
-  . apply ClapM.bind_wellFormed
-    . apply h_action.wellFormed
-    . apply h_function.wellFormed
-
--- TODO generalize
-lemma convertsM_map_FB_FArray
-  {len}
-  (action : ClapM p FB)
-  (f : FB → Vector FB len)
-  (state)
-  {action_val : Bool}
-  (f_val : Bool → Vector Bool len)
-  (h_action : FB.ConvertsM action state action_val)
-  (h_f_val : FArray.Converts len
-    (action.getState state)
-    (f (action.getResult state.numAlloc state.σ))
-    (f_val action_val)
-  )
-:
-  ConvertsM (f <$> action) state (f_val action_val)
-:= by
-  constructor
-  . simp
-    apply h_f_val
-  . rewrite [ClapM.map_wellFormed]
-    apply h_action.wellFormed
-
-lemma convertsM'_map_FB_FArray
-  {k}
-  (action : ClapM p FB)
-  (f : FB → Vector FB k)
-  (state)
-  {action_val : Bool}
-  (f_val : Bool → Vector Bool k)
-  (h_action : FB.ConvertsM action state action_val)
-  (h_f_val : FArray.Converts'
-    (action.getState state)
-    (f (action.getResult state.numAlloc state.σ))
-    (f_val action_val)
-  )
-:
-  ConvertsM' (f <$> action) state (f_val action_val)
-:= by
-  constructor
-  . simp
-    apply h_f_val
-  . rewrite [ClapM.map_wellFormed]
-    apply h_action.wellFormed
-
--- lemma convertsM_map_FB_FArray
---   {len}
---   (action : ClapM p FB)
---   (f : FB → Vector FB len)
---   (varStore : VarStore p)
---   (numAlloc : ℕ)
---   (σ : HashConsSt p)
---   {action_val : Bool}
---   (f_val : Bool → Vector Bool len)
---   (h_action : FArray.ConvertsM action varStore numAlloc σ action_val)
---   (h_f_val : FArray.Converts len
---     (action.getVarStore varStore numAlloc σ)
---     (action.getHashConsState numAlloc σ)
---     (action.getNumAlloc numAlloc σ)
---     (f (action.getResult numAlloc σ))
---     (f_val action_val)
---   )
--- :
---   ConvertsM (f <$> action) varStore numAlloc σ (f_val action_val)
--- := by
---   constructor
---   . simp
---     apply h_f_val
---   . rewrite [ClapM.map_wellFormed]
---     apply h_action.wellFormed
-
-@[aesop safe]
-lemma convertsM_pure
-        {state : ClapMState p}
-        {k : ℕ}
-        {x : FArray k}
-        {val : Vector Bool k}
-        (h : FArray.Converts k state x val)
-  : ConvertsM (pure x) state val := by
-  constructor
-  · simpa
-  · grind
-
-@[simp]
-lemma converts_empty
-        {state : ClapMState p}
-  : Converts 0 state #v[] #v[] := by
-  constructor
-  · simp
-  · grind
-  · grind
-
-@[aesop safe]
-lemma convertsM'_pure
-        {k}
-        {state : ClapMState p}
-        {x : Vector ExprRef k}
-        {val : Vector Bool k}
-        (h : FArray.Converts' state x val)
-  : ConvertsM' (pure x) state val := by
-  constructor
-  · simpa
-  · grind
-
-@[simp]
-lemma converts'_empty
-        {state : ClapMState p}
-  : Converts' state #v[] #v[] := by
-  constructor
-  . simp
-  · simp
-  · grind
-  · grind
-
-lemma converts_push
-  {k : ℕ}
-  {state : ClapMState p}
-  {exprs : Vector FB k}
-  {expr : FB}
-  {vals : Vector Bool k}
-  {val : Bool}
-  (h_exprs : FArray.Converts k state exprs vals)
-  (h_expr : FB.Converts state expr val)
-:
-  FArray.Converts (k + 1) state (exprs.push expr) (vals.push val)
-:= by
-  obtain ⟨exprs_varSet, exprs_wellFormed, exprs_result⟩ := h_exprs
-  obtain ⟨expr_varSet, expr_wellFormed, expr_result⟩ := h_expr
-  simp at *
-  constructor
-  all_goals {
-    intro i
-    simp
-    rewrite [Vector.getElem_push]
-    split
-    . specialize_all ⟨i.val, by assumption⟩
-      grind
-    . grind
-  }
-
-lemma converts'_push
-  {k}
-  {state : ClapMState p}
-  {exprs : Vector FB k}
-  {expr : FB}
-  {vals : Vector Bool k}
-  {val : Bool}
-  (h_exprs : FArray.Converts' state exprs vals)
-  (h_expr : FB.Converts state expr val)
-:
-  FArray.Converts' state (exprs.push expr) (vals.push val)
-:= by
-  obtain ⟨exprs_length, exprs_varSet, exprs_wellFormed, exprs_result⟩ := h_exprs
-  obtain ⟨expr_lengh, expr_varSet, expr_wellFormed, expr_result⟩ := h_expr
-  simp at *
-  constructor
-  . intro i
-    simp [Vector.getElem_push]
-    split
-    . exact exprs_varSet ⟨i.val, by grind⟩
-    . assumption
-  . intro i
-    simp [Vector.getElem_push]
-    split
-    . exact exprs_wellFormed ⟨i.val, by grind⟩
-    . assumption
-  . intro i
-    simp [Vector.getElem_push]
-    split
-    . exact exprs_result ⟨i.val, by grind⟩
-    . assumption
-  . grind
-
-end FArray
-
-namespace FList
-
-def Converts'
-  (state : ClapMState p)
-  (exprs : List FB)
-  (val : List Bool)
-:= Clap.Converts'
-  (fun l : List Bool ↦ l.map fun x ↦ if x then 1 else 0)
-  state
-  exprs
-  val
-
-structure ConvertsM'
-  (action : ClapM p (List FB))
-  (state)
-  (val : List Bool)
-: Prop where
-  result : Converts'
-    (action.getState state)
-    (action.getResult state.numAlloc state.σ)
-    val
-  wellFormed : action.wellFormed state.numAlloc state.varStore state.σ
-
-@[aesop safe]
-lemma convertsM'_pure
-        {state : ClapMState p}
-        {x : List FB}
-        {val : List Bool}
-        (h : FList.Converts' state x val)
-  : ConvertsM' (pure x) state val := by
-  constructor
-  · simpa
-  · grind
-
-@[simp]
-lemma converts'_empty
-        {state : ClapMState p}
-  : Converts' state [] [] := by
-  constructor
-  . simp
-  · simp
-  · grind
-  · grind
-
-@[aesop unsafe apply, grind =>]
-lemma converts'_skip_F
-  {skip : ClapM p F} {state}
-  {val' : ZMod p} {expr : List FB} {val : List Bool}
-  (h_skip : F.ConvertsM skip state val')
-  (h : FList.Converts' state expr val) :
-  FList.Converts' (skip.getState state)
-             expr
-             val := toIdeal_run_of_toIdeal' _ h_skip.wellFormed h
-
-@[aesop unsafe apply, grind =>]
-lemma converts'_skip_FB
-  {skip : ClapM p FB} {state}
-  {val' : Bool} {expr : List FB} {val : List Bool}
-  (h_skip : FB.ConvertsM skip state val')
-  (h : FList.Converts' state expr val) :
-  FList.Converts' (skip.getState state)
-             expr
-             val := toIdeal_run_of_toIdeal' _ h_skip.wellFormed h
-
-lemma converts'_append
-  {state : ClapMState p}
-  {exprs1 exprs2 : List FB}
-  {vals1 vals2 : List Bool}
-  (h_exprs1 : FList.Converts' state exprs1 vals1)
-  (h_exprs2 : FList.Converts' state exprs2 vals2)
-:
-  FList.Converts' state (exprs1 ++ exprs2) (vals1 ++ vals2)
-:= by
-  obtain ⟨exprs1_length, exprs1_varSet, exprs1_wellFormed, exprs1_result⟩ := h_exprs1
-  obtain ⟨exprs2_lengh, exprs2_varSet, exprs2_wellFormed, exprs2_result⟩ := h_exprs2
-  simp at *
-  constructor
-  . intro i
-    simp [List.getElem_append]
-    split
-    . exact exprs1_varSet ⟨i.val, by grind⟩
-    . exact exprs2_varSet ⟨_, by grind⟩
-  . intro i
-    simp [List.getElem_append]
-    split
-    . exact exprs1_wellFormed ⟨i.val, by grind⟩
-    . exact exprs2_wellFormed ⟨_, by grind⟩
-  . intro i
-    simp [List.getElem_append, exprs1_length]
-    split
-    . exact exprs1_result ⟨i.val, by grind⟩
-    . exact exprs2_result ⟨_, by grind⟩
-  . grind
-
-lemma converts'_of_converts_FB
-  {state : ClapMState p}
-  {exprs}
-  {vals}
-  (h_length : exprs.length = vals.length)
-  (h_converts : ∀ i : Fin exprs.length, FB.Converts state exprs[i] vals[i])
-:
-  FList.Converts' state exprs vals
-:= by
-  constructor
-  . intro i
-    have := (h_converts i).varSet_wf
-    simp at this
-    assumption
-  . intro i
-    have := (h_converts i).expr_wf
-    simp at this
-    assumption
-  . intro i
-    have := (h_converts i).value_eq
-    simp at this
-    simp [this]
-  . grind
-
-lemma converts'_singleton_of_converts_FB
-  {state : ClapMState p}
-  {expr}
-  {val}
-  (h_converts : FB.Converts state expr val)
-:
-  FList.Converts' state [expr] [val]
-:= by
-  apply converts'_of_converts_FB
-  . simpa
-  . simp
-
-end FList
-
-@[simp, grind =]
-lemma getState_map
-  {α β}
-  {state}
-  (action : ClapM p α)
-  (f : α → β)
-:
-  (f <$> action).getState state =
-  action.getState state
-:= by
-  grind [ClapM.getState]
-
-lemma FArray.convertsM'_of_convertsM'_toList
-  {k}
-  {action : ClapM p (Vector FB k)}
-  {state}
-  {val : Vector Bool k}
-  (h : FList.ConvertsM' (Vector.toList <$> action) state val.toList)
-:
-  FArray.ConvertsM' action state val
-:= by
-  constructor
-  . grind [FArray.Converts', FList.ConvertsM', FList.Converts']
-  . grind [FList.ConvertsM']
-
-
--- h_idx : F.Converts varStore σ numAlloc #v[idx] idx_val
--- h_tail : FArray.ConvertsM' mapM varStore numAlloc σ (List.map (fun a => a == idx_val.val) tail.reverse)
-
-@[aesop unsafe apply, grind =>]
-lemma F.converts_skip_FArray
-  {k}
-  {skip : ClapM p (Vector FB k)} {state}
-  {val' : Vector Bool k} {expr : F} {val : ZMod p}
-  (h_skip : FArray.ConvertsM' skip state val')
-  (h : F.Converts state expr val) :
-  F.Converts (skip.getState state)
-             expr
-             val := toIdeal_run_of_toIdeal' _ h_skip.wellFormed h
-
-@[aesop unsafe apply, grind =>]
-lemma F.converts_skip_F
-  {skip : ClapM p F} {state : ClapMState p}
-  {val' : ZMod p} {expr : F} {val : ZMod p}
-  (h_skip : F.ConvertsM skip state val')
-  (h : F.Converts state expr val) :
-  F.Converts (skip.getState state)
-             expr
-             val := toIdeal_run_of_toIdeal' _ h_skip.wellFormed h
-
-@[aesop unsafe apply, grind =>]
-lemma F.converts_skip_FB
-  {skip : ClapM p FB} {state} {val' : Bool} {expr : F} {val : ZMod p}
-  (h_skip : FB.ConvertsM skip state val')
-  (h : F.Converts state expr val) :
-  F.Converts (skip.getState state)
-             expr
-             val := toIdeal_run_of_toIdeal' _ h_skip.wellFormed h
-
-lemma F.converts_skip_FList
-  {skip : ClapM p (List FB)} {state} {val' : List Bool} {expr : F} {val : ZMod p}
-  (h_skip : FList.ConvertsM' skip state val')
-  (h : F.Converts state expr val) :
-  F.Converts (skip.getState state)
-             expr
-             val := toIdeal_run_of_toIdeal' _ h_skip.wellFormed h
-
-@[grind =]
-lemma deref_idxOf_of_mem
-  {cacheExpr : CacheExpr p}
-  {σ : HashConsSt p}
-  (h_mem : cacheExpr ∈ σ.exprs)
-:
-  *⦃σ.exprs.idxOf cacheExpr, σ⦄ = cacheExpr
-:= by
-  grind
-
-@[simp, grind =]
-lemma deref_mkVar_eq_some
-  {idx : ℕ}
-  {σ : HashConsSt p}
-:
-  *⦃(HashConsM.mkVar idx).getResult σ, (HashConsM.mkVar idx).getHashConsState σ⦄ =
-  .some (CacheExpr.v idx)
-:= by
-  grind [=HashConsM.mkVar]
-
-@[simp, grind =]
-lemma varSet_mkVar
-  {idx : ℕ}
-  {σ : HashConsSt p}
-:
-  ⦃(HashConsM.mkVar idx).getResult σ, (HashConsM.mkVar idx).getHashConsState σ⦄.varSet =
-  {idx}
-:= by
-  unfold Expr.varSet
-  grind
-
-@[simp, grind! .]
-lemma lt_getNumAlloc_isZero
-  {numAlloc : ℕ}
-  {σ : HashConsSt p}
-  {a : ExprRef}
-:
-  numAlloc < (isZero a).getNumAlloc numAlloc σ
-:= by
-  simp [isZero]
-
-namespace isZero
-
-lemma wellFormed {e! : ExprRef} {state} {value : ZMod p}
-  (h : F.Converts state e! value)
-:
-  (isZero e!).wellFormed state.numAlloc state.varStore state.σ
-:= by
-  obtain ⟨h_varSet, h_wellFormed, h_result⟩ := h
-  simp at *
-  apply wellFormed_isZero
-  . grind
-  . have : [state.varStore|⦃e!, state.σ⦄].isSome = true := by grind
-    grind
-  . grind
-
-lemma converts
-  [p.AtLeastTwo]
-  {state}
-  {a : F}
-  {a_val : ZMod p}
-  (h_a : F.Converts state a a_val)
-:
-  FB.Converts
-    ((isZero a).getState state)
-    ((isZero a).getResult state.numAlloc state.σ)
-    (a_val == 0)
-:= by
-  obtain ⟨a_length, a_varSet, a_wellFormed, a_result⟩ := h_a
-  obtain ⟨varStore, σ, numAlloc⟩ := state
-  simp [ClapM.getState]
-  constructor <;> simp at *
-  . intro i h_i
-    grind [=isZero, ClapM.getState]
-  . simp [isZero]
-    rw [Expr.wellFormed_iff_isSome, deref_mkVar_eq_some]
-    rfl
-  . simp [isZero, HashConsM.mkVar]
-    simp [HashConsM.getHashConsState_saveExpr_of_wellFormed,
-          HashConsM.getResult_saveExpr_of_wellFormed]
-    split
-    · rw [eval_eq_evalRec (by grind)]
-      unfold Expr.evalRec
-      grind
-    · rw [eval_eq_evalRec (by grind)]
-      rw [evalRec_eq_of_deref_eq_some_v (idx := numAlloc)]
-      · simp
-        rw [eval_eq_evalRec (by grind)] at a_result ⊢
-        rw [←evalRec_of_wellFormed_of_prefix] at ⊢
-        · rw [a_result]
-          grind
-        · grind
-        · grind
-      · grind
-
-lemma convertsM
-  [p.AtLeastTwo]
-  {state}
-  {a : F}
-  {a_val : ZMod p}
-  (h_a : F.Converts state a a_val)
-:
-  FB.ConvertsM (isZero a)
-    state
-    (a_val == 0)
-where
-  result := converts h_a
-  wellFormed := wellFormed h_a
-
--- structure ClapM' (p) where
---   cmd : ClapM p FB
---   val : Bool
---   varStore : VarStore p
---   numAlloc : ℕ
---   σ : HashConsSt p
---   spec : FB.ConvertsM cmd varStore numAlloc σ val
-
--- def IsZero' (p : ℕ) [p.AtLeastTwo] (a : F) (a_val : ZMod p)
---   (h_a : F.Converts varStore σ numAlloc #v[a] a_val)
--- : ClapM' p where
---   cmd := isZero a
---   val := a_val == 0
---   spec varStore numAlloc σ := @convertsM p _ varStore numAlloc σ a a_val
-
-
-
-
-def spec [p.AtLeastTwo]
-  {a : F} {state : ClapMState p} {a_val}
-  (h: (F.Converts state a a_val))
-:
-  FB.Spec (isZero a) state
-where
-  spec := a_val == 0
-  converts := convertsM h
-
-end isZero
-
-
-namespace mkSub
-
-lemma converts
-   {state}
-   {a b : ExprRef}
-   {a_val b_val : ZMod p}
-   (h_a : F.Converts state a a_val)
-   (h_b : F.Converts state b b_val)
-:
-  F.Converts
-    (ClapM.getState (liftM (HashConsM.mkSub (p := p) a b)) state)
-    (ClapM.getResult (liftM (HashConsM.mkSub (p := p) a b)) state.numAlloc state.σ)
-    (a_val - b_val)
-:= by
-  simp [ClapM.getState]
-  obtain ⟨a_length, a_varSet, a_wellFormed, a_result⟩ := h_a
-  obtain ⟨b_length, b_varSet, b_wellFormed, b_result⟩ := h_b
-  constructor <;>
-  simp at *
-  . grind [=Expr.varSet_wellFormed]
-  . grind
-  . simp [HashConsM.mkSub]
-    rewrite [HashConsM.getResult_saveExpr_of_wellFormed]
-    . rewrite [HashConsM.getHashConsState_saveExpr_of_wellFormed (by grind)]
-      . split <;> rewrite [eval_eq_evalRec (by grind)]
-        . rewrite [evalRec_eq_of_deref_eq_some_sub (deref_idxOf_of_mem (by assumption))]
-          dsimp
-          rewrite [
-            ←eval_eq_evalRec (by grind),
-            ←eval_eq_evalRec (by grind),
-            a_result,
-            b_result
-          ]
-          rfl
-        . rewrite [evalRec_eq_of_deref_eq_some_sub (Expr.deref_mk_size_push)]
-          dsimp
-          rewrite [
-            ←evalRec_of_wellFormed_of_prefix (σ := state.σ) (by grind) (by grind),
-            ←evalRec_of_wellFormed_of_prefix (σ := state.σ) (σ' := HashConsSt.pushExpr _ _ _) (by grind) (by grind),
-            ←eval_eq_evalRec (by grind),
-            ←eval_eq_evalRec (by grind),
-            a_result,
-            b_result
-          ]
-          rfl
-    . grind
-
-lemma convertsM
-  {state}
-  {a b : ExprRef}
-  {a_val b_val : ZMod p}
-  (h_a : F.Converts state a a_val)
-  (h_b : F.Converts state b b_val)
-:
-  F.ConvertsM (liftM (HashConsM.mkSub (p := p) a b)) state (a_val - b_val)
-where
-  result := converts h_a h_b
-  wellFormed := ClapM.wellFormed_liftM_of_hashConsM_wellFormed HashConsM.wellFormed_mkSub
-
-def spec
-  {a b : F} {state : ClapMState p} {a_val b_val}
-  (h_a: (F.Converts state a a_val))
-  (h_b: (F.Converts state b b_val))
-:
-  F.Spec state
-where
-  action := (liftM (HashConsM.mkSub (p := p) a b))
-  spec := a_val - b_val
-  converts := convertsM h_a h_b
-
-end mkSub
-
-namespace eq
-
-lemma convertsM
-  [p.AtLeastTwo]
-  {state}
-  {a b : F}
-  {a_val b_val : ZMod p}
-  (h_a : F.Converts state a a_val)
-  (h_b : F.Converts state b b_val)
-:
-  FB.ConvertsM (eq a b) state (a_val == b_val)
-:= by
-  unfold eq
-  apply FB.convertsM_of_convertsM_eq (a_val- b_val == 0)
-  . exact FB.convertsM_bind _ _ _ (λ x => x == (0 : ZMod p))
-      (mkSub.convertsM h_a h_b)
-      (isZero.convertsM (mkSub.convertsM h_a h_b).result)
-  . grind
-
--- def spec [p.AtLeastTwo]
---   {a b : F} {varStore : VarStore p} {numAlloc} {σ} {a_val} {b_val}
---   (h : (F.Converts varStore σ numAlloc #v[a] a_val))
---   (h : (F.Converts varStore σ numAlloc #v[b] b_val))
--- :
---   FB.Spec (eq a b) varStore numAlloc σ
--- where
---   spec := a_val == b_val
---   converts := by
---     unfold eq
---     --
-
-end eq
-
-namespace MkConstant
-
-@[simp]
-lemma convertsM
-  {state}
-  {x : ZMod p}
-:
-  F.ConvertsM (liftM (HashConsM.mkConstant (p := p) x)) state x
-:= by
-  constructor
-  · simp [ClapM.getState]
-    simp_rw [HashConsM.getResult_mkConstant, HashConsM.getHashConsState_mkConstant]
-    unfold F.Converts
-    constructor <;> simp
-    · grind [=Expr.varSet, =Expr.varSet_wellFormed]
-    · grind
-    · rw [eval_eq_evalRec (by grind)]
-      grind
-  · grind
-
-def spec
-  (x : ZMod p)
-  (state : ClapMState p)
-:
-  F.Spec state
-where
-  action := (liftM (HashConsM.mkConstant (p := p) x))
-  spec := x
-  converts := convertsM
-
--- TODO, see if this can be done generally?
-lemma fold_spec {x : ZMod p} (state : ClapMState p):
-  (liftM (HashConsM.mkConstant (p := p) x)) =
-  (spec x state).action
-:= rfl
-
-end MkConstant
-
-/--
-This one for any `LawfulMonad` sure was fun.
--/
-@[simp, grind =]
-lemma _root_.Vector.mapM_singleton'
-  {α}
-  {len : α}
-  (f : α → ClapM p FB)
-:
-  #v[len].mapM f =
-  f len >>= fun x => pure #v[x]
-:= by
-  unfold Vector.mapM
-  cbv
-  simp [WriterT.run]
-  funext
-  simp [StateT.bind]
-  cbv
-
-namespace MapM
-
-lemma _root_.Vector.take_append_last
-  {α}
-  {len : ℕ}
-  {vec : Vector α (len + 1)}
-:
-  ((vec.take len).cast (m := len) (by grind)) ++ #v[vec[len]] =
-  vec
-:= by
-  simp
-  ext
-  expose_names
-  have := Vector.getElem_append (n := len) (m := 1) (ys := #v[vec[len]]) (xs := vec.pop) (i := i) (by grind)
-  rewrite [this]
-  aesop (add safe (by grind))
-
-lemma _root_.Vector.mapM_succ
-  {α}
-  {len : ℕ}
-  {vec : Vector α (len + 1)}
-  (f : α → ClapM p FB)
-:
-  vec.mapM f =
-  (vec.pop.mapM f) >>= λ v => (λ x => v.push x) <$> f vec[len]
-:= by
-  rewrite [←Vector.take_append_last (vec:=vec)]
-  rw [Vector.mapM_append]
-  simp
-  have := Vector.take_append_last (vec:=vec)
-  simp at this
-  congr
-  . exact this.symm
-  . funext vecM
-    congr
-    exact this.symm
-
-end MapM
-
 namespace oneHotRaw
 
--- TODO generalize
-lemma convertsM'_map_FArray_FArray
+omit [p.AtLeastTwo] in
+lemma convertsM_map_FArray_FArray
   {k1 k2}
   (action : ClapM p (Vector FB k1))
   (f : Vector FB k1 → Vector FB k2)
   (state)
   {action_val : Vector Bool k1}
   (f_val : Vector Bool k1 → Vector Bool k2)
-  (h_action : FArray.ConvertsM' action state action_val)
-  (h_f_val : FArray.Converts'
+  (h_action : FArray.ConvertsM action state action_val)
+  (h_f_val : FArray.Converts
     (action.getState state)
     (f (action.getResult state.numAlloc state.σ))
     (f_val action_val)
   )
 :
-  FArray.ConvertsM' (f <$> action) state (f_val action_val)
+  FArray.ConvertsM (f <$> action) state (f_val action_val)
 := by
   constructor
   . simp
     apply h_f_val
   . rewrite [ClapM.map_wellFormed]
     apply h_action.wellFormed
+  . grind [ClapM.runAndEval, h_action.constraints]
 
+omit [p.AtLeastTwo] in
 @[grind .]
 lemma bind_wellFormed'
   {α β}
@@ -1279,7 +1246,6 @@ lemma bind_wellFormed'
 
 
 lemma convertsM_but_sane?
-  [p.AtLeastTwo]
   {state}
   {len : ℕ}
   {idx : F}
@@ -1287,9 +1253,9 @@ lemma convertsM_but_sane?
   (h_idx : F.Converts state idx idx_val)
   (h_len : len < p)
 :
-  FArray.ConvertsM' (oneHotRaw len idx) state (Vector.ofFn (λ x => x.val == idx_val.val))
+  FArray.ConvertsM (oneHotRaw len idx) state (Vector.ofFn (λ x => x.val == idx_val.val))
 := by
-  apply FArray.convertsM'_of_convertsM'_toList
+  apply FArray.convertsM_of_convertsM_toList
   simp_rw [toList_map_oneHotRaw_eq_oneHotRaw']
   unfold oneHotRaw' oneHotRaw'_aux
 
@@ -1302,10 +1268,10 @@ lemma convertsM_but_sane?
   ]
 
   set list := List.range' 0 len
-  have : ∀ x ∈ list, x < p := by grind
+  have not_this : ∀ x ∈ list, x < p := by grind
   clear_value list
 
-  rw [←list.reverse_reverse] at this ⊢
+  rw [←list.reverse_reverse] at not_this ⊢
   set list := list.reverse
   clear_value list
   induction' eq_ih : list.length with len h_len generalizing list
@@ -1319,8 +1285,11 @@ lemma convertsM_but_sane?
       simp at h_len
 
       -- assert that our previous state still holds after the mapM
-      obtain ⟨h_mapM_result, h_wellFormed⟩ := h_len
-      apply F.converts_skip_FList ⟨h_mapM_result, h_wellFormed⟩ at h_idx
+      have := h_len
+      have h_mapM_result := FList.converts_of_convertsM this
+      have h_wellFormed := this.wellFormed
+      have h_constraints1 := this.constraints
+      apply F.converts_skip this at h_idx
       set mapM := List.mapM
           (fun i => do
             let idx_val ← liftM (HashConsM.mkConstant (i : ZMod p))
@@ -1328,36 +1297,51 @@ lemma convertsM_but_sane?
           tl.reverse
       set mapM_result := mapM.getResult state.numAlloc state.σ
       set state := mapM.getState state
+      clear this
 
       -- Get ConvertsM for mkConstant and assert that previous state still holds
-      obtain ⟨h_a, h_wellFormed⟩ := @MkConstant.convertsM p state hd
-      apply F.converts_skip_F ⟨h_a, h_wellFormed⟩ at h_idx
-      apply FList.converts'_skip_F ⟨h_a, h_wellFormed⟩ at h_mapM_result
+      have := @MkConstant.convertsM p state hd
+      have h_a := F.converts_of_convertsM this
+      have h_wellFormed := this.wellFormed
+      have h_constraints2 := this.constraints
+      apply F.converts_skip this at h_idx
+      apply FList.converts_skip this at h_mapM_result
       set mkConst := (liftM (n := ClapM p) (HashConsM.mkConstant (p := p) (hd : ZMod p)))
       set c_result := mkConst.getResult state.numAlloc state.σ
       set state := mkConst.getState state
+      clear this
 
       -- Get ConvertsM for eq and assert that previous state still holds
-      obtain ⟨h_eq, h_wellFormed⟩ := eq.convertsM h_idx h_a
-      apply F.converts_skip_FB ⟨h_eq, h_wellFormed⟩ at h_idx
-      apply FList.converts'_skip_FB ⟨h_eq, h_wellFormed⟩ at h_mapM_result
+      have := eq.convertsM h_idx h_a
+      have h_eq := FB.converts_of_convertsM this
+      have h_wellFormed := this.wellFormed
+      have h_constraints2 := this.constraints
+      apply F.converts_skip this at h_idx
+      apply FList.converts_skip this at h_mapM_result
       set eq := eq (p := p) idx c_result
       set eq_result := eq.getResult state.numAlloc state.σ
       set eq_state := eq.getState state
+      clear this
 
       -- Apply the Functor map to the result of our eq, leaving the state unaffected
-      have h_eq_map := FList.converts'_append
+      have h_eq_map := FList.converts_append
         h_mapM_result
-        (FList.converts'_singleton_of_converts_FB h_eq)
+        (FList.converts_singleton_of_converts_FB h_eq)
+
+      simp at *
+          -- We've reached the end of the function, so strip away the boilerplate and prove
+                -- that the canonical spec matches our hand written one
+
 
       -- We've reached the end of the function, so strip away the boilerplate and prove
       -- that the canonical spec matches our hand written one
       constructor
-      . convert h_eq_map
+      . unfold FList.Converts at h_eq_map
+        convert h_eq_map
         . grind [ClapM.getState]
         . grind [ClapM.getState]
         . -- Spec proof
-          rewrite [←ZMod.val_cast_of_lt (a := hd) (this hd (by grind))]
+          rewrite [←ZMod.val_cast_of_lt (a := hd) (not_this hd (by grind))]
           simp only [ZMod.val_natCast, beq_eq_beq]
           apply Iff.intro
           . intro h
@@ -1365,311 +1349,303 @@ lemma convertsM_but_sane?
           . intro h
             simp [h]
       . grind
-
-
-#exit
-#exit
-#exot
-
-
-
-  -- apply Clap.ClapM.bind_wellFormed
-  -- · grind
-  -- . rcases h_a with ⟨h₁, h₂, h₃⟩
-  --   rcases h_b with ⟨h₄, h₅, h₆⟩
-  --   simp
-  --   apply wellFormed_isZero
-  --   · simp at *
-  --     grind
-  --   · simp at *
-  --     intros val hval
-  --     rw [Std.ExtTreeMap.mem_iff_isSome_getElem?]
-  --     -- rw [eval_eq_evalRec (by grind)] at h₃ h₆
-  --     have : [varStore | ⦃a[0], σ⦄].isSome := by grind
-  --     have : [varStore | ⦃b[0], σ⦄].isSome := by grind
-  --     grind -- `Option.isSome_of_eq_some` is useless, had to go via `wellFormed_mem_varStore_of_evalRec_eq_some`... yikes?
-  --   · simp at *
-  --     grind [=Expr.varSet_wellFormed]
-
-lemma matches_spec
-  [p.AtLeastTwo]
-  {varStore : VarStore p}
-  {numAlloc : ℕ}
-  {σ : HashConsSt p}
-  (a b : F)
-  (a_val b_val : ZMod p)
-  (h_a_wf_σ : (Expr.mk a σ).wellFormed)
-  (h_b_wf_σ : (Expr.mk b σ).wellFormed)
-  (h_a_wf : [varStore|Expr.mk a σ].isSome = true)
-  (h_a_val : [varStore,σ|a].get h_a_wf = a_val)
-  (h_b_wf : [varStore|Expr.mk b σ].isSome = true)
-  (h_b_val : [varStore,σ|b].get h_b_wf = b_val)
-  -- (h_σ_a : Expr.varSet_wellFormed ⟨a, σ⟩ numAlloc)
-  -- (h_σ_b : Expr.varSet_wellFormed ⟨b, σ⟩ numAlloc)
-:
-  F.matches_spec
-    varStore
-    numAlloc
-    σ
-    (eq a b)
-    (a_val == b_val)
-    FB.Convert.toIdeal
-:= by
-  dsimp [F.matches_spec]
-  set aExpr : Expr _ := ⟨a, σ⟩
-  have : aExpr.wellFormed := by grind
-
-  set bExpr : Expr _ := ⟨b, σ⟩
-  have : bExpr.wellFormed := by grind
-
-  set subCExpr : CacheExpr p := .binary_op (p := p) a b .sub
-  have subCExprWf : subCExpr.wellFormed σ.size := by grind
-
-  set f := a.eq b (p := p) with hf
-
-  have : f.getCircuit numAlloc σ = #[Gate.isZero (σ.exprs.idxOf subCExpr)] := by
-    grind [eq]
-
-  set σ₁ := (HashConsM.mkSub a b).getHashConsState σ with eq_σ₁
-  have eq₁ : subCExpr ∈ σ₁.exprs := by grind
-  set σ₂ := f.getHashConsState numAlloc σ with eq_σ₂
-  have eq₃ : subCExpr ∈ σ₂.exprs := by grind [=eq]
-  have eq₄ : .v numAlloc ∈ σ₂.exprs := by grind [=eq]
-  have : f.getResult numAlloc σ = (HashConsM.mkVar numAlloc).getResult σ₁ := by
-    grind [=eq]
-  rw [this]
-  let res₀ := (HashConsM.mkSub a b).getResult σ
-  set res₁ := (HashConsM.mkVar numAlloc).getResult σ₁ with eq_res₁
-  let res₀_val := [varStore| ⦃res₀, (HashConsM.mkVar numAlloc).getHashConsState σ₁⦄]
-  have : f.getVarStore varStore numAlloc σ =
-         varStore.insert numAlloc (if res₀_val = some 0 then 1 else 0) := by
-    rw [hf]
-    unfold eq
-    rw [ClapM.getVarStore_bind_of_wellFormed (by simp)]
-    swap
-    simp
-    apply wellFormed_isZero (by grind) (by grind)
-    swap
-    simp [res₀_val, res₀, eq_σ₁]
-
-  sorry
-
-end eq
-
-namespace oneHotRaw
-
-def spec (len : ℕ) (idx : ℕ) : Vector Bool len :=
-  (Vector.range len).map (fun (i:ℕ) ↦ idx == i)
-
-opaque Convert.toIdeal {len : ℕ} (varStore : VarStore p) (σ : HashConsSt p) (result : Vector FB len) : Option (Vector Bool len)
-
-lemma Convert.toIdeal_push
-  {len : ℕ} {vec : Vector Bool len} {extra : FB} {val : Bool}
-  {varStore : VarStore p}
-  {σ : HashConsSt p}
-  {result : Vector FB len}
-  (h_base : Convert.toIdeal varStore σ result = .some vec)
-  (h_extra : FB.Convert.toIdeal varStore σ extra = .some val)
-:
-  Convert.toIdeal varStore σ (result.push extra) = .some (vec.push val)
-:= by
-  done
-
--- lemma Vector.mapM_append {p} {α β} {n} {n'}
---     {f : α → ClapM p β} {xs : Vector α n} :
---     xs.mapM f =
---     (λ numAlloc σ => (((), ), ))
--- := by
---   done
-
-@[grind .]
-lemma getVarStore_precedes_of_wellFormed
-  {α}
-  {Γ : VarStore p}
-  {numAlloc : ℕ}
-  {σ σ': HashConsSt p}
-  {action : ClapM p α}
-:
-  [σ'|Γ ⊑ action.getVarStore Γ numAlloc σ]
-:= by
-  unfold ClapM.getVarStore
-  grind
-
-lemma wellFormed
-  [p.AtLeastTwo]
-  {len : ℕ}
-  {idx : F}
-  {varStore : VarStore p}
-  {numAlloc : ℕ}
-  {σ : HashConsSt p}
-  {idx_val : ℕ}
-  (h_idx_val : (F.Convert.toIdeal varStore σ idx).map ZMod.val = .some idx_val)
-  (h_idx_varSet : Expr.varSet_wellFormed ⟨idx, σ⟩ numAlloc)
-:
-  (oneHotRaw len idx).wellFormed numAlloc varStore σ
-:= by
-  have h_isSome : (F.Convert.toIdeal varStore σ idx).isSome = true := by grind
-  induction' len with len h_len
-  . have : Vector.range 0 = #v[] := rfl
-    simp [oneHotRaw, this]
-  . have :
-      oneHotRaw (len + 1) idx =
-      do
-        let vec ← oneHotRaw len idx
-        let idx_val ← liftM (HashConsM.mkConstant (p := p) len)
-        let elem ← F.eq (p := p) idx idx_val
-        return vec.push elem
-    := by
-      simp [oneHotRaw, Vector.range_succ, Vector.mapM_append, -Vector.append_singleton]
-      set v := Vector.mapM
-          (fun i => do
-            let idx_val ← liftM (HashConsM.mkConstant (i : ZMod p))
-            idx.eq (p := p) idx_val)
-          (Vector.range len)
-      simp
-    simp [this]
-    apply ClapM.bind_wellFormed (by grind)
-    apply ClapM.bind_wellFormed
-    . grind
-    . apply eq.wellFormed <;> simp
-      . have h_lt: idx < σ.size := by grind [wellFormed_of_toIdeal_isSome]
-        have h_le : σ.size ≤ ((oneHotRaw len idx).getHashConsState numAlloc σ).size := by grind
-        apply lt_of_lt_of_le (lt_of_lt_of_le h_lt h_le)
-        rewrite [HashConsM.getHashConsState_mkConstant]
-        grind
-      . grind [HashConsM.getResult_lt_getHashConsState_size_mkConstant] -- grind why
-      . rewrite [←ClapM.getVarStore]
-        have := isSome_eval_of_isSome_toIdeal h_isSome
-        apply isSome_eval_of_isSome_eval_precedes (Γ₁ := varStore)
-        . apply isSome_eval_of_prefix _ this
-          . grind
-          . grind
-          . exact wellFormed_of_toIdeal_isSome h_isSome
-        . have := wellFormed_of_toIdeal_isSome h_isSome
-          grind
-        . simp
-          grind
-      . unfold Expr.varSet_wellFormed
-        rewrite [varSet.varSet_mk_eq_of_prefix (σ1 := σ)]
-        . grind
-        . grind [wellFormed_of_toIdeal_isSome]
-        . apply Array.isPrefixOf_trans h_len.2.2
-          apply HashConsM.wellFormed_mkConstant
-      . grind [Expr.varSet_wellFormed]
-
---TODO prove using eq.matches_spec
---this may require adding to F.matches_spec, or defining properties about Convert.toIdeal
---in either case, the goal is to reach a fixed point where the same properties are known about the two Convert.toIdeal functions,
---and the same F.matches_spec is being used for eq and proven for oneHotRaw
-lemma matches_spec
-  [p.AtLeastTwo]
-  {len : ℕ}
-  {idx : F}
-  {varStore : VarStore p}
-  {numAlloc : ℕ}
-  {σ : HashConsSt p}
-  {idx_val : ℕ}
-  (h_idx_val : F.Convert.toIdeal varStore σ idx idx_val)
-  (h_idx_varSet : Expr.varSet_wellFormed ⟨idx, σ⟩ numAlloc)
-:
-  F.matches_spec
-    varStore
-    numAlloc
-    σ
-    (oneHotRaw len idx)
-    (spec len idx_val)
-    Convert.toIdeal
-:= by
-  unfold F.matches_spec
-  set f := oneHotRaw len idx (p := p) with eq
-  unfold oneHotRaw at eq
-  set range_vec := Vector.range len
-  induction' len with len ih
-  · have : Vector.range 0 = #v[] := rfl
-    simp [this, range_vec] at eq
-    subst f
-    simp [eq]
-    unfold spec
-    simp [this]
-    have todoLater₁ : Convert.toIdeal varStore σ #v[] = some #v[] := sorry
-    exact todoLater₁
-  · simp at ih
-    specialize ih (by rfl)
-    have :
-      oneHotRaw (len + 1) idx =
-      do
-        let vec ← oneHotRaw len idx
-        let idx_val ← liftM (HashConsM.mkConstant (p := p) len)
-        let elem ← F.eq (p := p) idx idx_val
-        return vec.push elem
-    := by
-      simp [oneHotRaw, Vector.range_succ, Vector.mapM_append, -Vector.append_singleton]
-      set v := Vector.mapM
-          (fun i => do
-            let idx_val ← liftM (HashConsM.mkConstant (i : ZMod p))
-            idx.eq (p := p) idx_val)
-          (Vector.range len)
-      simp
-    unfold oneHotRaw at this
-    simp [range_vec, this] at eq
-    rewrite [←oneHotRaw.eq_def] at eq
-    have : spec (len + 1) idx_val = spec len idx_val ++ #v[idx_val == len] := by
-      unfold spec
-      simp [Vector.range_succ]
-    rw [this]
-    have :
-      Convert.toIdeal
-        (f.getVarStore varStore numAlloc σ)
-        (f.getHashConsState numAlloc σ)
-        (f.getResult numAlloc σ) =
-      (Convert.toIdeal
-        ((oneHotRaw len idx).getVarStore varStore numAlloc σ)
-        ((oneHotRaw len idx).getHashConsState numAlloc σ)
-        ((oneHotRaw len idx).getResult numAlloc σ)).get (by grind) ++
-      #v[(F.Convert.toIdeal
-          ((oneHotRaw len idx).getVarStore varStore numAlloc σ)
-          ((oneHotRaw len idx).getHashConsState numAlloc σ)
-          idx).map (ZMod.val) == .some len
-      ]
-    := by
-      simp [ih]
-      have :
-        f.getResult numAlloc σ =
-        ((oneHotRaw len idx).getResult numAlloc σ).push
-          ((idx.eq ((HashConsM.mkConstant (len : ZMod p)).getResult ((oneHotRaw len idx).getHashConsState numAlloc σ))).getResult
-          ((oneHotRaw len idx).getNumAlloc numAlloc σ)
-          ((HashConsM.mkConstant (len : ZMod p)).getHashConsState ((oneHotRaw len idx).getHashConsState numAlloc σ)))
-      := by
-        simp [eq]
-      rewrite [this]; clear this
-      rewrite [Convert.toIdeal_push]
-      . rfl
-      . simp [eq]
-        rewrite [ClapM.getVarStore_bind_of_wellFormed (wellFormed h_idx_val h_idx_varSet)]
-        . done
-        . apply ClapM.bind_wellFormed
-          . grind
-          . simp
-            apply F.eq.wellFormed
-            . have h_toIdeal : (F.Convert.toIdeal varStore σ idx).isSome = true := by aesop
-              have := wellFormed_of_toIdeal_isSome h_toIdeal
-
-              done
-          done
-        done
-      done
-
-    simp [this, ih]
-    rewrite [toIdeal_eq_toIdeal_of_wellFormed, h_idx_val]
-    . aesop
-    . apply wellFormed_of_toIdeal_isSome (varStore := varStore)
-      grind
-    . grind
-    . exact wellFormed h_idx_val h_idx_varSet
-  done
+      . grind [ClapM.getState]
 
 end oneHotRaw
+end OneHotRaw
 
-end F
+section assert_eq
+
+def assert_eq (a b : F) : ClapM p Unit := do
+  let diff ← HashConsM.mkSub (p := p) a b
+  eq0 diff
+
+namespace assert_eq
+
+lemma convertsM
+  [p.AtLeastTwo]
+  {a b} {val}
+  {state : ClapMState p}
+  (h_a : F.Converts state a val)
+  (h_b : F.Converts state b val)
+:
+  FUnit.ConvertsM (assert_eq a b) state ()
+:= by
+  unfold assert_eq
+
+  have := mkSub.convertsM h_a h_b
+  have h_wf := this.wellFormed
+  have h_constraints := this.constraints
+  simp only [ClapM.map_wellFormed] at h_wf
+  simp at this
+  have := eq0.convertsM (F.converts_of_convertsM this)
+  have h_wf := this.wellFormed
+  have h_constraints := this.constraints
+  unfold FUnit.ConvertsM at this
+  constructor
+  . convert this.result using 1
+    . grind
+    . grind
+  . grind
+  . grind [ClapM.getState]
+
+end assert_eq
+end assert_eq
+
+section sum
+
+open HashConsM in
+def FArray.sum' {k} (init : F) (vals : FArray k) : ClapM p F := do
+  vals.foldlM (λ x y => liftM (mkAdd (p := p) x y)) init
+
+namespace FArray.sum'
+
+lemma convertsM
+  {k}
+  {state : ClapMState p}
+  {f_vals : FArray k}
+  {vals : Vector Bool k}
+  {init : F}
+  (h_vals : FArray.Converts state f_vals vals)
+  (h_init : F.Converts state init 0)
+:
+  F.ConvertsM (f_vals.sum' init) state (vals.map (λ x => if x then (1: ZMod p) else 0)).sum
+:= by
+  unfold sum'
+
+  induction' k with k h_k
+  . have (init : ExprRef) : Vector.foldlM (λ x y => liftM (n := ClapM p) (HashConsM.mkAdd (p := p) x y)) init f_vals = pure init := by
+      convert Vector.foldlM_empty
+      obtain ⟨⟨_⟩, _⟩ := f_vals
+      grind
+    simp [this]
+    have : vals = #v[] := by grind
+    simp [this]
+    constructor
+    . unfold F.Converts at h_init
+      simp [ClapM.getState]
+      grind [cases ClapMState]
+    . grind
+    . simp [ClapM.runAndEval]
+  . have := (FArray.converts_cast (k2 := k) (FArray.converts_pop h_vals) (by trivial))
+    set fvals_base := Vector.cast (m := k) (by trivial) f_vals.pop
+    set vals_base := Vector.cast (m := k) (by trivial) vals.pop
+
+    have := @h_k fvals_base vals_base this
+    have h_fvals_base := F.converts_of_convertsM this
+    have h_wellFormed := this.wellFormed
+    have h_constraints2 := this.constraints
+    apply FArray.converts_skip this at h_vals
+    set foldlM := Vector.foldlM (fun x y => liftM (n := ClapM p) (HashConsM.mkAdd (p := p) x y)) init fvals_base
+    set foldl_result := foldlM.getResult state.numAlloc state.σ
+    set state := foldlM.getState state
+    simp at *
+    clear this
+
+    have : f_vals = fvals_base.push f_vals[k] := by
+      ext
+      rewrite [Vector.getElem_push]
+      split
+      . simp [fvals_base]
+      . grind
+    rewrite [this]
+    simp [Vector.foldlM_push]
+
+    have h_fvals_k := F.converts_of_FB_converts (FArray.converts_getElem h_vals (Nat.lt_succ_self k))
+
+    have := mkAdd.convertsM h_fvals_base h_fvals_k
+    have h_add := F.converts_of_convertsM this
+    have h_wellFormed := this.wellFormed
+    have h_constraints2 := this.constraints
+    set add := liftM (n := ClapM p) (HashConsM.mkAdd (p := p) foldl_result f_vals[k])
+    set add_result := add.getResult state.numAlloc state.σ
+    set state := add.getState state
+    simp at *
+    clear this
+
+    constructor
+    . unfold F.Converts at h_add
+      convert h_add
+      . grind
+      . grind [ClapM.getState]
+      . have : vals = vals_base.push vals[k] := by
+          ext
+          rewrite [Vector.getElem_push]
+          split
+          . simp [vals_base]
+          . grind
+        rewrite [this]
+        simp
+    . grind
+    . grind [ClapM.getState]
+
+end FArray.sum'
+
+
+
+open HashConsM in
+def FArray.sum {k} (vals : FArray k) : ClapM p F := do
+  vals.foldlM (λ x y => liftM (mkAdd (p := p) x y)) (←liftM (mkConstant (0 : ZMod p)))
+
+namespace FArray.sum
+
+lemma convertsM
+  {k}
+  {state : ClapMState p}
+  {f_vals : FArray k}
+  {vals : Vector Bool k}
+  (h_vals : FArray.Converts state f_vals vals)
+:
+  F.ConvertsM (f_vals.sum) state (vals.map (λ x => if x then (1: ZMod p) else 0)).sum
+:= by
+  unfold sum
+  simp [←sum'.eq_def]
+
+  have := @MkConstant.convertsM p state 0
+  have h_zero := F.converts_of_convertsM this
+  have h_wf := this.wellFormed
+  have h_constraints := this.constraints
+  apply FArray.converts_skip this at h_vals
+  set mkZero := liftM (n := ClapM p) (HashConsM.mkConstant (p := p) 0)
+  set mkZero_result := mkZero.getResult state.numAlloc state.σ
+  set mkZero_state := mkZero.getState state
+  simp at *
+
+  have := sum'.convertsM h_vals h_zero
+  have h_sum' := F.converts_of_convertsM this
+  have h_wf := this.wellFormed
+  have h_constraints := this.constraints
+
+  constructor
+  . unfold F.Converts at h_sum'
+    convert h_sum'
+    . grind
+    . grind [ClapM.getState]
+  . grind
+  . grind [ClapM.getState]
+
+end FArray.sum
+end sum
+
+section singleOneArray
+
+/-- Returns a one-hot bit mask of length `len` with a 1 at index `idx` and 0s elsewhere. Only satisfiable when `0 ≤ idx < len`. -/
+def singleOneArray [p.AtLeastTwo] (len : ℕ) (idx : F) : ClapM p (FArray len) := do
+  let out ← oneHotRaw len idx
+  let s : F ← out.sum
+  assert_eq s (←liftM (HashConsM.mkConstant (1 : ZMod p)))
+  return out
+
+namespace singleOneArray
+
+lemma convertsM
+  [p.AtLeastTwo]
+  {len : ℕ}
+  {idx : F}
+  {state}
+  {idx_val : ZMod p}
+  (h_idx : F.Converts state idx idx_val)
+  (h_len : len < p)
+  (h_idx_val : idx_val.val < len)
+:
+  FArray.ConvertsM (singleOneArray len idx) state (Vector.ofFn (λ x => x.val == idx_val.val))
+:= by
+  unfold singleOneArray
+
+  have := oneHotRaw.convertsM_but_sane? h_idx h_len
+  have h_oneHot := FArray.converts_of_convertsM this
+  have h_wellFormed := this.wellFormed
+  have h_constraints2 := this.constraints
+  apply F.converts_skip this at h_idx
+  simp [-toList_map_oneHotRaw_eq_oneHotRaw'] at *
+  set result := (oneHotRaw len idx).getResult state.numAlloc state.σ
+  set state := (oneHotRaw len idx).getState state
+  clear this
+
+  have := FArray.sum.convertsM h_oneHot
+  have h_sum := F.converts_of_convertsM this
+  have h_wellFormed := this.wellFormed
+  have h_constraints2 := this.constraints
+  apply F.converts_skip this at h_idx
+  apply FArray.converts_skip this at h_oneHot
+  simp at *
+  set sum := result.sum.getResult state.numAlloc state.σ
+  set state := result.sum.getState state
+  clear this
+
+  have := @MkConstant.convertsM p state 1
+  have h_one := F.converts_of_convertsM this
+  have h_wellFormed := this.wellFormed
+  have h_constraints2 := this.constraints
+  apply F.converts_skip this at h_idx
+  apply FArray.converts_skip this at h_oneHot
+  apply F.converts_skip this at h_sum
+  simp at h_idx h_oneHot h_sum
+  set mkOne := liftM (n := ClapM p) (HashConsM.mkConstant (p := p) 1)
+  set one := mkOne.getResult state.numAlloc state.σ
+  set state := mkOne.getState state
+  clear this
+
+  have : (Vector.ofFn ((fun x => if x = true then 1 else 0) ∘ (λ x : Fin len => x == idx_val.val))).sum = (1 : ZMod p) := by
+    clear *-h_len h_idx_val
+    induction' len with len ih
+    . grind
+    . specialize ih (by grind)
+      rewrite [Vector.ofFn_succ]
+      by_cases h: idx_val.val = len
+      . simp [h]
+        clear ih
+        have (i : Fin len) : (i.val = len) = false := by grind
+        simp [this]
+        clear *-len
+        unfold Vector.ofFn
+        simp
+        induction' len with len ih'
+        . set x := Array.ofFn _
+          have : x = #[] := rfl
+          grind
+        . rewrite [Array.ofFn_succ]
+          grind
+      . specialize ih (by grind)
+        simp
+        rewrite [ite_cond_eq_false]
+        . simp
+          convert ih
+          grind
+        . grind
+
+  have h_sum : F.Converts state sum 1 := by
+    convert h_sum
+    rw [this]
+
+  have := assert_eq.convertsM h_sum h_one
+  have h_wellFormed := this.wellFormed
+  have h_constraints2 := this.constraints
+  apply F.converts_skip this at h_idx
+  apply FArray.converts_skip this at h_oneHot
+  apply F.converts_skip this at h_sum
+  apply F.converts_skip this at h_one
+  simp at h_idx h_oneHot h_sum h_one
+  set assert := assert_eq sum one
+  set assert_result := assert.getResult state.numAlloc state.σ
+  set state := assert.getState state
+  clear this
+
+  constructor
+  . unfold FArray.Converts at h_oneHot
+    convert h_oneHot
+    . grind
+    . grind
+  . grind
+  . grind [ClapM.getState]
+
+
+
+end singleOneArray
+
+end singleOneArray
+
+
+
 
 end Clap.Lang
